ott_coq/destination_calculus_notations.v
@@ -17,7 +17,7 @@ Notation "'hvars©(' C ')'" := (hvars_ectxs C) (at level 0, no associativity).
 (* Terms : 40-59 *)
 Notation "'ᵥ₎' v" := (term_Val v) (at level 40, no associativity).
 Notation "'ₓ₎' x" := (term_Var x) (at level 40, no associativity).
-Notation "t  u" := (term_App t u) (at level 42, left associativity, u at next level).
+Notation "t $ u" := (term_App t u) (at level 42, left associativity, u at next level).
 Notation "t 'ᵗ;' u" := (term_PatU t u) (at level 45, right associativity, u at next level).
 Notation "t 'caseˢ' m '{Inl' x1 ⟼ u1 , 'Inr' x2 ⟼ u2 '}'" := (term_PatS t m x1 u1 x2 u2) (at level 59, m at level 29, x1 at level 19, x2 at level 19, u1 at level 59, u2 at level 59, right associativity).
 Notation "t 'caseᵖ' m 'ᵗ(' x1 ',' x2 ')' ⟼ u" := (term_PatP t m x1 x2 u) (at level 59, m at level 29, x1 at level 19, x2 at level 19, u at level 59, right associativity).
